src/SymEval.v
@@ -7,33 +7,40 @@ Set Implicit Arguments.
 Notation "m [ k |--> v ]" := (add k v m) (at level 0).
 Notation "m [ k |-> v ]" := (m [k |--> {| objVal := v |}]) (at level 0).
 Notation "v === m .[ k ]" := (find k m = Some {| objVal := v |}) (at level 70).
+Notation "_=== m .[ k ]" := (find k m = None) (at level 70).
 
 Notation "m ~{ k |-> v }" := ((fun a => if weq a k then v else m a) : type (Vector (Bit _) _)) (at level 0).
 
-Fixpoint SymSemAction k (a : Action type k) (rs rs' : RegsT) (cs : CallsT) (kf : RegsT -> CallsT -> type k -> Prop) : Prop :=
+Fixpoint SymSemAction k (a : Action type k) (rs rsNotWritable rs' : RegsT) (cs : CallsT) (kf : RegsT -> CallsT -> type k -> Prop) : Prop :=
   match a with
   | MCall meth s marg cont =>
     forall mret,
       cs meth = None
-      /\ SymSemAction (cont mret) rs rs' cs[meth |-> (evalExpr marg, mret)] kf
+      /\ SymSemAction (cont mret) rs rsNotWritable rs' cs[meth |-> (evalExpr marg, mret)] kf
   | Let_ _ e cont =>
-    SymSemAction (cont (evalExpr e)) rs rs' cs kf
+    SymSemAction (cont (evalExpr e)) rs rsNotWritable rs' cs kf
   | ReadReg r _ cont =>
     exists regV,
       regV === rs.[r]
-      /\ SymSemAction (cont regV) rs rs' cs kf
+      /\ SymSemAction (cont regV) rs rsNotWritable rs' cs kf
   | WriteReg r _ e cont =>
-    rs' r = None
-    /\ SymSemAction cont rs rs'[r |-> evalExpr e] cs kf
+    match rsNotWritable r with
+    | Some _ => True
+    | None =>
+      match rs' r with
+      | None => SymSemAction cont rs rsNotWritable rs'[r |-> evalExpr e] cs kf
+      | Some _ => False
+      end
+    end
   | IfElse p _ a a' cont =>
     if evalExpr p
-    then SymSemAction a rs rs' cs (fun rs'' cs' rv =>
-                                     SymSemAction (cont rv) rs rs'' cs' kf)
-    else SymSemAction a' rs rs' cs (fun rs'' cs' rv =>
-                                      SymSemAction (cont rv) rs rs'' cs' kf)
+    then SymSemAction a rs rsNotWritable rs' cs (fun rs'' cs' rv =>
+                                                   SymSemAction (cont rv) rs rsNotWritable rs'' cs' kf)
+    else SymSemAction a' rs rsNotWritable rs' cs (fun rs'' cs' rv =>
+                                                    SymSemAction (cont rv) rs rsNotWritable rs'' cs' kf)
   | Assert_ p cont =>
     evalExpr p = true
-    -> SymSemAction cont rs rs' cs kf
+    -> SymSemAction cont rs rsNotWritable rs' cs kf
                                  
   | Return e => kf rs' cs (evalExpr e)
   end.
@@ -71,35 +78,77 @@ Proof.
   auto.
 Qed.
 
-Lemma SymSemAction_sound' : forall k (a : Action type k) rs rs' cs' rv,
+Lemma Disj_union1 : forall A (m1 m2 m : @Map A),
+  Disj (union m1 m2) m
+  -> Disj m1 m.
+Proof.
+  intros; intro k.
+  specialize (H k).
+  unfold find, union, unionL in *; intuition idtac.
+  destruct (m1 k); auto.
+Qed.
+
+Lemma Disj_union2 : forall A (m1 m2 m : @Map A),
+  Disj (union m1 m2) m
+  -> Disj m2 m.
+Proof.
+  intros; intro k.
+  specialize (H k).
+  unfold find, union, unionL in *; intuition idtac.
+  destruct (m1 k); auto; discriminate.
+Qed.
+
+Lemma Disj_add : forall A (m1 m2 : @Map A) k v,
+  Disj m1[k |--> v] m2
+  -> Disj m1 m2.
+Proof.
+  intros; intro k0.
+  specialize (H k0).
+  unfold find, add, unionL in *; intuition idtac.
+  destruct (string_dec k k0); subst.
+  rewrite string_dec_eq in *; discriminate.
+  rewrite string_dec_neq in * by tauto; tauto.
+Qed.
+
+Hint Immediate Disj_union1 Disj_union2 Disj_add.
+
+Lemma SymSemAction_sound' : forall k (a : Action type k) rs rsNotWritable rs' cs' rv,
   SemAction rs a rs' cs' rv
-  -> forall rs'' cs kf, SymSemAction a rs rs'' cs kf
+  -> forall rs'' cs kf, SymSemAction a rs rsNotWritable rs'' cs kf
+    -> Disj rs' rsNotWritable
     -> kf (union rs'' rs') (union cs cs') rv.
 Proof.
   induction 1; simpl; intuition.
 
   specialize (H0 mret); intuition.
-  eapply IHSemAction in H2.
-  subst.
-  rewrite union_add by assumption; auto.
+  eapply IHSemAction in H3; auto.
+  subst; rewrite union_add by assumption; auto.
 
   destruct H0; intuition.
-  specialize (double_find _ _ HRegVal H1); intro; subst.
+  specialize (double_find _ _ HRegVal H2); intro; subst.
   apply IHSemAction; auto.
 
-  apply IHSemAction in H2.
   subst.
+  generalize (H1 r).
+  unfold find at 2.
+  intuition.
+  rewrite find_add_1 in H3; discriminate.
+  rewrite H3 in H0.
+  destruct (rs'' r) eqn:Hrs''; intuition.
+  apply IHSemAction in H0; eauto.
   rewrite union_add in * by assumption; auto.
-
+  
   rewrite HTrue in *.
-  apply IHSemAction1 in H1.
-  apply IHSemAction2 in H1.
+  subst.
+  apply IHSemAction1 in H1; eauto.
+  apply IHSemAction2 in H1; eauto.
   subst.
   repeat rewrite union_assoc; auto.
 
   rewrite HFalse in *.
-  apply IHSemAction1 in H1.
-  apply IHSemAction2 in H1.
+  subst.
+  apply IHSemAction1 in H1; eauto.
+  apply IHSemAction2 in H1; eauto.
   subst.
   repeat rewrite union_assoc; auto.
 
@@ -108,15 +157,14 @@ Proof.
   repeat rewrite union_empty_2; congruence.
 Qed.
 
-Theorem SymSemAction_sound : forall k (a : Action type k) rs rs' cs rv,
+Theorem SymSemAction_sound : forall k (a : Action type k) rs rsNotWritable rs' cs rv,
   SemAction rs a rs' cs rv
-  -> forall kf, SymSemAction a rs empty empty kf
+  -> forall kf, SymSemAction a rs rsNotWritable empty empty kf
+    -> Disj rs' rsNotWritable
     -> kf rs' cs rv.
 Proof.
   intros.
-  apply (SymSemAction_sound' H) in H0.
-  repeat rewrite union_empty_1 in H0.
-  auto.
+  apply (SymSemAction_sound' H) in H0; auto.
 Qed.
 
 (* Considering method calls only.  We later build a version that considers trying a rule first, too. *)
@@ -127,7 +175,7 @@ Fixpoint SymSemMod_methods (dms : list (DefMethT type)) (rs rs' : RegsT) (dmeth 
   | meth :: dms' =>
     SymSemMod_methods dms' rs rs' dmeth cmeth kf
     /\ find (attrName meth) dmeth = None
-    /\ forall argV, SymSemAction (objVal (attrType meth) argV) rs rs' cmeth
+    /\ forall argV, SymSemAction (objVal (attrType meth) argV) rs rs' rs' cmeth
                                  (fun rs'' cmeth' retV =>
                                     SymSemMod_methods dms' rs rs'' dmeth[attrName meth |-> (argV, retV)] cmeth' kf)
   end.
@@ -140,9 +188,21 @@ Fixpoint SymSemMod (dms : list (DefMethT type)) (rules : list (Attribute (Action
            /\ SymSemMod_methods dms rs rs' dmeth cmeth (kf None)
   | rule :: rules' =>
     SymSemMod dms rules' rs rs' dmeth cmeth kf
-    /\ SymSemAction (attrType rule) rs rs' cmeth
+    /\ SymSemAction (attrType rule) rs rs' rs' cmeth
                     (fun rs'' cmeth' _ =>
                        SymSemMod_methods dms rs rs'' dmeth cmeth' (kf (Some (attrName rule))))
+  end.
+
+Fixpoint SymMatchCalls (ls : list string) (cmeth dmeth : CallsT) (P : Prop) : Prop :=
+  match ls with
+  | nil => P
+  | x :: ls' =>
+    let rest := SymMatchCalls ls' cmeth dmeth P in
+    match find x cmeth, find x dmeth with
+    | Some _, None => True
+    | Some call1, Some call2 => call1 = call2 -> rest
+    | _, _ => rest
+    end
   end.
 
 Fixpoint SymLtsStep (ms : Modules type) (rs : RegsT)
@@ -161,35 +221,53 @@ Fixpoint SymLtsStep (ms : Modules type) (rs : RegsT)
                      match match rm, rm' with Some _, Some _ => None | Some _, _ => Some rm | _, _ => Some rm' end with
                      | None => True
                      | Some rm'' =>
-                       kf rm'' (disjUnion rs1 rs2 (map (@attrName _) (getRegInits m1)))
-                          (disjUnion (complement dmeth1 (getCmsMod m2))
-                                     (complement dmeth2 (getCmsMod m1))
-                                     (listSub (getDmsMod m1) (getCmsMod m2)))
-                          (disjUnion (complement cmeth1 (getDmsMod m2))
-                                     (complement cmeth2 (getDmsMod m1))
-                                     (listSub (getCmsMod m1) (getDmsMod m2)))
+                       SymMatchCalls (getDmsMod m2) cmeth1 dmeth2
+                                     (SymMatchCalls (getDmsMod m1) cmeth2 dmeth1
+                                                    (kf rm'' (disjUnion rs1 rs2 (map (@attrName _)
+                                                                                     (getRegInits m1)))
+                                                        (disjUnion (complement dmeth1 (getCmsMod m2))
+                                                                   (complement dmeth2 (getCmsMod m1))
+                                                                   (listSub (getDmsMod m1) (getCmsMod m2)))
+                                                        (disjUnion (complement cmeth1 (getDmsMod m2))
+                                                                   (complement cmeth2 (getDmsMod m1))
+                                                                   (listSub (getCmsMod m1) (getDmsMod m2)))))
                      end))
   end.
+
+Theorem Disj_uniony : forall A (a b c : @Map A),
+  Disj a b
+  -> Disj (union a b) c
+  -> Disj b (union c a).
+Proof.
+  unfold Disj, union, unionL, find; intros.
+  specialize (H k).
+  specialize (H0 k).
+  intuition auto.
+  rewrite H1 in *; tauto.
+  rewrite H; tauto.
+Qed.
+
+Hint Immediate Disj_uniony.
 
 Theorem SymSemMod_methods_sound : forall rules rs rm rs' meths dmeth cmeth,
   SemMod rules rs rm rs' meths dmeth cmeth
   -> forall rs'' dmeth' cmeth' kf, SymSemMod_methods meths rs rs'' dmeth' cmeth' kf
     -> rm = None
+    -> Disj rs' rs''
     -> kf (union rs'' rs') (union dmeth' dmeth) (union cmeth' cmeth).
 Proof.
   induction 1; simpl; intuition subst; try discriminate.
 
   repeat rewrite union_empty_2; auto.
 
-  eapply SymSemAction_sound' in HAction.
-  2: eauto.
+  eapply SymSemAction_sound' in HAction; eauto.
   simpl in *.
-  apply IHSemMod in HAction; auto.
+  apply IHSemMod in HAction; eauto.
   repeat rewrite union_assoc.
   rewrite union_add by assumption.
   assumption.
 
-  apply IHSemMod in H2; auto.
+  eapply IHSemMod in H2; eauto.
 Qed.
 
 Lemma SysSemMod_base : forall dms rules rs rs' dmeth cmeth kf,
@@ -203,7 +281,7 @@ Qed.
 Lemma SysSemMod_ind : forall dms rule rules rs rs' dmeth cmeth kf,
   SymSemMod dms rules rs rs' dmeth cmeth kf
   -> In rule rules
-  -> SymSemAction (attrType rule) rs rs' cmeth
+  -> SymSemAction (attrType rule) rs rs' rs' cmeth
                   (fun rs'' cmeth' _ => SymSemMod_methods dms rs rs'' dmeth cmeth' (kf (Some (attrName rule)))).
 Proof.
   induction rules; simpl; intuition (subst; auto).
@@ -212,6 +290,7 @@ Qed.
 Theorem SymSemMod_sound : forall rules rs rm rs' meths dmeth cmeth,
   SemMod rules rs rm rs' meths dmeth cmeth
   -> forall rs'' dmeth' cmeth' kf, SymSemMod meths rules rs rs'' dmeth' cmeth' kf
+    -> Disj rs' rs''
     -> kf rm (union rs'' rs') (union dmeth' dmeth) (union cmeth' cmeth).
 Proof.
   induction 1; simpl; intuition subst.
@@ -256,6 +335,20 @@ Proof.
   destruct (m2 k); intuition congruence.
 Qed.
 
+Lemma SymMatchCalls_sound : forall cmeth dmeth P ls,
+  SymMatchCalls ls cmeth dmeth P
+  -> (forall x, In x ls -> InMap x cmeth -> find x dmeth = find x cmeth)
+  -> P.
+Proof.
+  induction ls; simpl; intuition.
+  generalize (H0 a); intuition.
+  unfold InMap in *.
+  destruct (find a cmeth).
+  rewrite H1 in * by discriminate.
+  auto.
+  destruct (find a cmeth); auto.
+Qed.
+
 Theorem SymLtsStep_sound : forall ms rm rs rs' dmeth cmeth,
   LtsStep ms rm rs rs' dmeth cmeth
   -> forall kf, SymLtsStep ms rs kf
@@ -275,7 +368,10 @@ Proof.
   apply IHLtsStep2 in H5.
   hnf in H3; simpl in H3; subst.
   hnf in H7; simpl in H7; subst.
+  hnf in H1; simpl in H1; intuition.
   hnf in H2; intuition subst.
-  destruct rm2; auto.
-  destruct rm1; auto.
+  destruct rm2; auto;
+  (eapply SymMatchCalls_sound; [ eapply SymMatchCalls_sound | .. ]; eauto).
+  destruct rm1; auto;
+  (eapply SymMatchCalls_sound; [ eapply SymMatchCalls_sound | .. ]; eauto).
 Qed.
