examples/SymEvalTest.v
@@ -1,0 +1,65 @@
+Require Import FunctionalExtensionality List String.
+Require Import Lib.Word Lib.Struct Lib.FnMap.
+Require Import Lts.Syntax Lts.Semantics Lts.Refinement Lts.SymEval Lts.SymEvalTac.
+
+Definition bar := MethodSig "bar"(Bit 1) : Bit 1.
+
+Theorem call_me : forall rm o n dm cm, LtsStep (ConcatMod (MODULE {
+                                                               Method "foo"() : Bit 1 :=
+                                                                 Call x <- bar($1);
+                                                                 Ret #x
+                                                          })
+                                                          (MODULE {
+                                                               Method "bar"(x : Bit 1) : Bit 1 :=
+                                                                 Ret #x
+                                                          }))
+                                               rm o n dm cm
+                                       -> forall r : Typed SignT, find "foo" dm = Some r
+                                         -> exists w, r = {| objType := Build_SignatureT (Bit 0) (Bit 1);
+                                                             objVal := (w, WO~1) |}.
+Proof.
+  do 6 intro.
+  SymEval.
+  eauto.
+Qed.
+
+Definition inc := MethodSig "inc"() : Void.
+Definition inc2 := MethodSig "inc2"() : Void.
+
+Theorem really_atomic : forall rm o n dm cm, LtsStep (ConcatMod (MODULE {
+                                                                     Register "r" : Bit 2 <- Default
+
+                                                                     with Method "inc"() : Void :=
+                                                                       Read r : Bit 2 <- "r";
+                                                                       Write "r" <- #r + $1;
+                                                                       Retv
+
+                                                                     with Method "inc2"() : Void :=
+                                                                       Read r : Bit 2 <- "r";
+                                                                       Write "r" <- #r + $2;
+                                                                       Retv
+                                                                })
+                                                                (MODULE {
+                                                                     Method "either"(b : Bool) : Void :=
+                                                                       If (#b) then
+                                                                         Call inc();
+                                                                         Retv
+                                                                       else
+                                                                         Call inc2();
+                                                                         Retv
+                                                                       as _;
+                                                                       Retv
+                                                                }))
+                                               rm o n dm cm
+                                       -> ($0 : type (Bit 2)) === o.["r"]
+                                       -> _=== n.["r"]
+                                          \/ ($1 : type (Bit 2)) === n.["r"]
+                                          \/ ($2 : type (Bit 2)) === n.["r"].
+Proof.
+  intros.
+  SymEval;
+    repeat match goal with
+           | [ |- context[if ?argV then _ else _] ] => destruct argV; SymEval_simpl
+           | [ |- exists x, _ = _ /\ _ ] => eexists; split; [ solve [ eauto ] | intuition idtac ]
+           end.
+Qed.
